mm0-lean/x86/hla.lean
@@ -28,10 +28,15 @@ structure hla.ok (H : hla) (k : config) : Prop :=
 
 def hla.config (H : hla) := {k // H.ok k}
 
+inductive mem_base : Type
+| abs (off : ℤ) : mem_base -- only valid for LEA arithmetic
+| mem (arena off : ℕ) : mem_base -- uses RIP-relative offset
+| reg : regnum → ℤ → mem_base
+
 inductive arg : Type
 | imm : qword → arg
 | reg : regnum → arg
-| mem : option scale_index → base → ℤ → arg
+| mem : option scale_index → mem_base → arg
 | label : ℕ → arg
 | llabel : ℕ → ℕ → arg
 
@@ -83,70 +88,79 @@ inductive assemble_label (H : hla) : arg → qword → Prop
   c.2.1.nth n = some q →
   assemble_label (arg.llabel i n) q
 
-def arg.imm_rm : arg → imm_rm → Prop
-| (arg.reg r) rm := imm_rm.rm (RM.reg r) = rm
-| (arg.mem ix b d) rm := imm_rm.rm (RM.mem ix b d) = rm
+def mem_base.to_base (H : hla) (rip : qword) : mem_base → base → qword → Prop
+| (mem_base.abs q) b off := b = base.none ∧ off = q
+| (mem_base.mem i a) b off := ∃ c,
+  H.mem.nth i = some c ∧
+  b = base.rip ∧ off = c.2.1 + a - rip
+| (mem_base.reg r q) b off := b = base.reg r ∧ off = q
+
+def arg.imm_rm (H : hla) (rip : qword) : arg → imm_rm → Prop
+| (arg.reg r) rm := rm = imm_rm.rm (RM.reg r)
+| (arg.mem ix b) rm := ∃ b' o,
+  mem_base.to_base H rip b b' o ∧
+  rm = imm_rm.rm (RM.mem ix b' o)
 | (arg.imm q) rm := imm_rm.imm q = rm
 | _ _ := false
 
-def arg.rm : arg → RM → Prop
-| (arg.reg r) rm := RM.reg r = rm
-| (arg.mem ix b d) rm := RM.mem ix b d = rm
-| _ _ := false
+def arg.imm_rm' (H : hla) (a : arg) : pstate config imm_rm :=
+pstate.assert $ λ k rm, a.imm_rm H k.rip rm
 
-theorem arg.rm_imm_rm {a rm} :
-  arg.rm a rm ↔ arg.imm_rm a (imm_rm.rm rm) :=
-by cases a; simp [arg.rm, arg.imm_rm]
+def arg.rm (H : hla) (rip : qword) (a : arg) (rm : RM) : Prop :=
+arg.imm_rm H rip a (imm_rm.rm rm)
 
-def assemble_ds (d s : arg) : dest_src → Prop
-| (dest_src.Rm_i rm q) := arg.rm d rm ∧ s = arg.imm q
-| (dest_src.Rm_r rm r) := arg.rm d rm ∧ s = arg.reg r
-| (dest_src.R_rm r rm) := arg.rm d (RM.reg r) ∧ arg.rm s rm
+def arg.rm' (H : hla) (a : arg) : pstate config RM :=
+pstate.assert $ λ k rm, a.rm H k.rip rm
+
+def assemble_ds (H : hla) (rip : qword) (d s : arg) : dest_src → Prop
+| (dest_src.Rm_i rm q) := arg.rm H rip d rm ∧ s = arg.imm q
+| (dest_src.Rm_r rm r) := arg.rm H rip d rm ∧ s = arg.reg r
+| (dest_src.R_rm r rm) := arg.rm H rip d (RM.reg r) ∧ arg.rm H rip s rm
 
 def code_pred := hla → list qword → qword → list byte → Prop
 
-def asm1.pred' : asm1 → ast → Prop
+def asm1.pred' (H : hla) (rip : qword) : asm1 → ast → Prop
 | (asm1.unop op sz a) v := ∃ rm,
-  a.rm rm ∧
+  a.rm H rip rm ∧
   ast.unop op sz rm = v
 | (asm1.binop op sz d s) v := ∃ ds,
-  assemble_ds d s ds ∧
+  assemble_ds H rip d s ds ∧
   ast.binop op sz ds = v
 | (asm1.mul sz a) v := ∃ rm,
-  a.rm rm ∧
+  a.rm H rip rm ∧
   ast.mul sz rm = v
 | (asm1.div sz a) v := ∃ rm,
-  a.rm rm ∧
+  a.rm H rip rm ∧
   ast.div sz rm = v
 | (asm1.lea sz d s) v := ∃ ds,
-  assemble_ds d s ds ∧
+  assemble_ds H rip d s ds ∧
   ast.lea sz ds = v
 | (asm1.movsx sz d s sz2) v := ∃ ds,
-  assemble_ds d s ds ∧
+  assemble_ds H rip d s ds ∧
   ast.movsx sz ds sz2 = v
 | (asm1.movzx sz d s sz2) v := ∃ ds,
-  assemble_ds d s ds ∧
+  assemble_ds H rip d s ds ∧
   ast.movzx sz ds sz2 = v
 | (asm1.xchg sz a r) v := ∃ rm,
-  a.rm rm ∧
+  a.rm H rip rm ∧
   ast.xchg sz rm r = v
 | (asm1.cmpxchg sz a r) v := ∃ rm,
-  a.rm rm ∧
+  a.rm H rip rm ∧
   ast.cmpxchg sz rm r = v
 | (asm1.xadd sz a r) v := ∃ rm,
-  a.rm rm ∧
+  a.rm H rip rm ∧
   ast.xadd sz rm r = v
 | (asm1.cmov c sz d s) v := ∃ ds,
-  assemble_ds d s ds ∧
+  assemble_ds H rip d s ds ∧
   ast.cmov c sz ds = v
 | (asm1.setcc c b a) v := ∃ rm,
-  a.rm rm ∧
+  a.rm H rip rm ∧
   ast.setcc c b rm = v
 | (asm1.push a) v := ∃ rm,
-  a.imm_rm rm ∧
+  a.imm_rm H rip rm ∧
   ast.push rm = v
 | (asm1.pop a) v := ∃ rm,
-  a.rm rm ∧
+  a.rm H rip rm ∧
   ast.pop rm = v
 | asm1.leave v := ast.leave = v
 | asm1.cmc v := ast.cmc = v
@@ -154,139 +168,330 @@ def asm1.pred' : asm1 → ast → Prop
 | asm1.stc v := ast.stc = v
 | asm1.syscall v := ast.syscall = v
 
-theorem arg.imm_rm.determ {a rm1 rm2} : arg.imm_rm a rm1 → a.imm_rm rm2 → rm1 = rm2 :=
-by cases a; rintro ⟨⟩ ⟨⟩; refl
+-- theorem arg.imm_rm.determ {a rm1 rm2} : arg.imm_rm a rm1 → a.imm_rm rm2 → rm1 = rm2 :=
+-- by cases a; rintro ⟨⟩ ⟨⟩; refl
 
-theorem arg.rm.determ {a rm1 rm2} : arg.rm a rm1 → arg.rm a rm2 → rm1 = rm2 :=
-by cases a; rintro ⟨⟩ ⟨⟩; refl
+-- theorem arg.rm.determ {a rm1 rm2} : arg.rm a rm1 → arg.rm a rm2 → rm1 = rm2 :=
+-- by cases a; rintro ⟨⟩ ⟨⟩; refl
 
-def arg.ea (k : config) (a : arg) (ea : EA) : Prop :=
-∃ rm, arg.imm_rm a rm ∧ imm_rm.ea k rm = ea
+-- def HLEA.hla_ok (H : hla) : EA → wsize → Prop
+-- | (EA.m q) sz := ∃ c, c ∈ H.mem ∧ _
+-- | _ sz := true
 
-theorem arg.ea.determ {k a ea1 ea2} : arg.ea k a ea1 → a.ea k ea2 → ea1 = ea2 :=
-by rintro ⟨_, h1, rfl⟩ ⟨_, h2, rfl⟩; cases h1.determ h2; refl
+inductive HLEA
+| i : qword → HLEA
+| r : regnum → HLEA
+| m : ℕ → ℕ → HLEA
+| abs : qword → HLEA
 
-theorem arg.imm_rm.ea {a rm k} (h : arg.imm_rm a rm) : arg.ea k a (rm.ea k) :=
-by cases a; cases h; exact ⟨_, rfl, rfl⟩
+def HLEA.to_ea (H : hla) : HLEA → EA → Prop
+| (HLEA.i q) ea := ea = EA.i q
+| (HLEA.r r) ea := ea = EA.r r
+| (HLEA.m i a) ea := ∃ c, H.mem.nth i = some c ∧ ea = EA.m (c.2.1 + a)
+| (HLEA.abs q) ea := ea = EA.m q
 
-theorem arg.rm.ea {a rm k} (h : arg.rm a rm) : arg.ea k a (rm.ea k) :=
-(arg.rm_imm_rm.1 h).ea
-
-theorem assemble_ds.src {d s ds k}
-  (h : assemble_ds d s ds) : arg.ea k s (ea_src k ds) :=
+theorem HLEA.to_ea.determ {H ea ea1 ea2}
+  (h1 : HLEA.to_ea H ea ea1) (h2 : HLEA.to_ea H ea ea2) : ea1 = ea2 :=
 begin
-  cases ds; cases h,
-  { subst s, exact ⟨_, rfl, rfl⟩ },
-  { subst s, refine ⟨_, rfl, rfl⟩ },
-  { exact h_right.ea },
+  cases ea; try { exact h1.trans h2.symm },
+  rcases h1 with ⟨c1, a1, rfl⟩, rcases h2 with ⟨c2, a2, rfl⟩,
+  cases a1.symm.trans a2, exact rfl
 end
 
-theorem assemble_ds.dest {d s ds k}
-  (h : assemble_ds d s ds) : arg.ea k d (ea_dest k ds) :=
-by cases ds; cases h; exact h_left.ea
+def HLEA.to_ea' (H : hla) (ea : HLEA) : pstate config EA :=
+pstate.assert $ λ _ ea', HLEA.to_ea H ea ea'
 
-def arg.read (k : config) (a : arg) (sz : wsize) (w : bitvec sz.to_nat) : Prop :=
-∃ ea, arg.ea k a ea ∧ ea.read k sz w
+-- def EA.hla_ok (H : hla) (ea : EA) (sz : wsize) : Prop :=
+-- ∃ ea', HLEA.ea H sz ea ea'
 
-def arg.readq (k : config) (a : arg) (sz : wsize) (q : qword) : Prop :=
-∃ ea, arg.ea k a ea ∧ ea.readq k sz q
+-- def arg.ea (k : config) (a : arg) (ea : EA) : Prop :=
+-- ∃ rm, arg.imm_rm a rm ∧ imm_rm.ea k rm = ea
 
-def arg.writeq (k : config) (a : arg) (sz : wsize) (q : qword) (k' : config) : Prop :=
-∃ ea, arg.ea k a ea ∧ ea.writeq k sz q k'
+def index_ea' (k : config) : option scale_index → ℤ
+| none := 0
+| (some ⟨s, i⟩) := nat.shiftl 1 s.to_nat * (k.regs i).to_int
 
-def asm1.exec (k k' : config) : asm1 → Prop
-| (asm1.unop op sz rm) := ∃ ea w,
-  arg.ea k rm ea ∧ ea.readq k sz w ∧
-  write_unop sz w ea op k k'
-| (asm1.binop op sz d s) := ∃ ea d' s',
-  arg.ea k d ea ∧ ea.readq k sz d' ∧
-  s.readq k sz s' ∧
-  write_binop sz ea d' s' op k k'
-| (asm1.mul sz r) := ∃ eax src k2,
-  (EA.EA_r RAX).readq k sz eax ∧
-  r.readq k sz src ∧
-  match sz with
-  | (wsize.Sz8 _) :=
-    (EA.EA_r RAX).writeq k wsize.Sz16 (eax * src) k2
-  | _ := ∃ k1,
-    let hi := bitvec.of_nat sz.to_nat
-      ((eax.to_nat * src.to_nat).shiftl sz.to_nat) in
-    (EA.EA_r RAX).writeq k sz (eax * src) k1 ∧
-    (EA.EA_r RDX).writeq k1 sz (EXTZ hi) k2
-  end ∧
-  erase_flags k2 k'
-| (asm1.div sz r) := ∃ eax edx d k1 k2,
-  (EA.EA_r RAX).readq k sz eax ∧
-  (EA.EA_r RDX).readq k sz edx ∧
-  let n := edx.to_nat * (2 ^ sz.to_nat) + eax.to_nat in
-  r.readq k sz d ∧
-  let d := bitvec.to_nat d in
-  d ≠ 0 ∧ n / d < 2 ^ sz.to_nat ∧
-  (EA.EA_r RAX).writeq k sz (bitvec.of_nat _ (n / d)) k1 ∧
-  (EA.EA_r RDX).writeq k1 sz (bitvec.of_nat _ (n % d)) k2 ∧
-  erase_flags k2 k'
-| (asm1.lea sz d s) := ∃ sea,
-  arg.ea k s sea ∧
-  d.writeq k sz sea.addr k'
-| (asm1.movsx sz1 d s sz2) := ∃ w,
-  s.read k sz1 w ∧
-  d.writeq k sz2 (EXTZ (EXTS w : bitvec sz2.to_nat)) k'
-| (asm1.movzx sz1 d s sz2) := ∃ w,
-  s.read k sz1 w ∧
-  d.writeq k sz2 (EXTZ w) k'
-| (asm1.xchg sz r n) := ∃ dst val_src val_dst k1,
-  let src := EA.EA_r n in
-  r.ea k dst ∧
-  src.readq k sz val_src ∧
-  dst.readq k sz val_dst ∧
-  src.writeq k sz val_dst k1 ∧
-  dst.writeq k1 sz val_src k'
-| (asm1.cmpxchg sz r n) := ∃ dst val_dst val_acc,
-  let src := EA.EA_r n, acc := EA.EA_r RAX in
-  r.ea k dst ∧
-  dst.readq k sz val_dst ∧
-  acc.readq k sz val_acc ∧
-  (do
-    write_binop sz src val_acc val_dst binop.cmp,
-    if val_acc = val_dst then
-      src.read' sz >>= dst.write' sz
-    else acc.write' sz val_dst) k k'
-| (asm1.xadd sz r n) := ∃ dst val_src val_dst k1,
-  let src := EA.EA_r n in
-  r.ea k dst ∧
-  src.readq k sz val_src ∧
-  dst.readq k sz val_dst ∧
-  src.writeq k sz val_dst k1 ∧
-  write_binop sz dst val_src val_dst binop.add k1 k'
-| (asm1.cmov c sz d s) :=
-  cond (c.read k.flags)
-    (∃ w, s.readq k sz w ∧ d.writeq k sz w k')
-    (k = k')
-| (asm1.setcc c b r) :=
-  r.writeq k (wsize.Sz8 b) (EXTZ $ bitvec.singleton $ c.read k.flags) k'
-| (asm1.push i) := ∃ i',
-  arg.imm_rm i i' ∧ push i' k k'
-| (asm1.pop r) := ∃ r',
-  arg.rm r r' ∧ pop r' k k'
-| asm1.leave :=
-  pop (RM.reg RBP) (k.set_reg RSP (k.regs RBP)) k'
-| asm1.clc := k' = {flags := {CF := ff, ..k.flags}, ..k}
-| asm1.cmc := k' = {flags := {CF := bnot k.flags.CF, ..k.flags}, ..k}
-| asm1.stc := k' = {flags := {CF := tt, ..k.flags}, ..k}
-| asm1.syscall := false
+@[simp] theorem index_ea'_coe {k ix} : (index_ea' k ix : qword) = index_ea k ix :=
+begin
+  cases ix, refl,
+  cases ix, simp [index_ea', index_ea, bitvec.coe_shl, bitvec.coe_to_int],
+end
+
+inductive mem_base.ea (H : hla) (k : config) (ix : ℤ) : mem_base → HLEA → Prop
+| abs (i) : mem_base.ea (mem_base.abs i) (HLEA.abs (ix + i : ℤ))
+| mem (i a a' : ℕ) : (ix + a : ℤ) = a' →
+  mem_base.ea (mem_base.mem i a) (HLEA.m i a')
+| reg (r off) (a' : ℕ) (i c) :
+  H.mem.nth i = some c →
+  ix + (k.regs r).to_int + off - c.2.1.to_nat = a' →
+  mem_base.ea (mem_base.reg r off) (HLEA.m i a')
+| reg_abs (r off) :
+  mem_base.ea (mem_base.reg r off) (HLEA.abs (ix + (k.regs r).to_int + off : ℤ))
+
+def arg.ea (H : hla) (k : config) : arg → HLEA → Prop
+| (arg.imm q) ea := ea = HLEA.i q
+| (arg.reg r) ea := ea = HLEA.r r
+| (arg.mem ix b) ea := mem_base.ea H k (index_ea' k ix) b ea
+| _ _ := false
+
+def arg.ea' (H : hla) (a : arg) : pstate config HLEA :=
+pstate.assert $ λ k ea, a.ea H k ea
+
+-- theorem arg.ea.determ {k a ea1 ea2} : arg.ea k a ea1 → a.ea k ea2 → ea1 = ea2 :=
+-- by rintro ⟨_, h1, rfl⟩ ⟨_, h2, rfl⟩; cases h1.determ h2; refl
+
+theorem arg.imm_rm.ea {H a rm k ea}
+  (h1 : arg.ea H k a ea)
+  (h2 : arg.imm_rm H k.rip a rm) : ea.to_ea H (rm.ea k) :=
+begin
+  cases a,
+  { cases h1, cases h2, exact rfl },
+  { cases h1, cases h2, exact rfl },
+  { rcases h2 with ⟨b, q, h, rfl⟩,
+    rcases h1 with i | ⟨i, a, a', h3⟩ |
+      ⟨r, off, a', i, c, h3, h4⟩ | ⟨r, off⟩;
+    dsimp [imm_rm.ea, RM.ea, HLEA.to_ea],
+    { rcases h with ⟨rfl, rfl⟩, simp [base.ea] },
+    { rcases h with ⟨c, h, rfl, rfl⟩,
+      refine ⟨_, h, _⟩,
+      have h3 := congr_arg (coe : ℤ → qword) h3, simp at h3, rw ← h3,
+      simp [base.ea], ring },
+    { rcases h with ⟨rfl, rfl⟩,
+      refine ⟨_, h3, _⟩,
+      have h4 := congr_arg (coe : ℤ → qword) h4, simp at h4, rw ← h4,
+      simp [base.ea, bitvec.coe_to_nat, bitvec.coe_to_int] },
+    { rcases h with ⟨rfl, rfl⟩, simp [base.ea, bitvec.coe_to_int] } },
+  { cases h1 },
+  { cases h1 }
+end
+
+theorem arg.rm.ea {H a rm k ea}
+  (h1 : arg.ea H k a ea)
+  (h2 : arg.rm H k.rip a rm) : ea.to_ea H (rm.ea k) :=
+arg.imm_rm.ea h1 h2
+
+theorem assemble_ds.src {H d s ds k ea}
+  (h : assemble_ds H (k:config).rip d s ds)
+  (h2 : arg.ea H k s ea) : ea.to_ea H (ea_src k ds) :=
+begin
+  cases ds; cases h,
+  { subst s, cases h2, exact rfl },
+  { subst s, cases h2, exact rfl },
+  { dsimp [ea_src], exact h_right.ea h2 },
+end
+
+theorem assemble_ds.dest {H d s ds k ea}
+  (h : assemble_ds H (k:config).rip d s ds)
+  (h2 : arg.ea H k d ea) : ea.to_ea H (ea_dest k ds) :=
+by cases ds; cases h; exact h_left.ea h2
+
+def HLEA.read (H : hla) (k : config) (sz : wsize) (w : bitvec sz.to_nat) : HLEA → Prop
+| (HLEA.i i) := w = EXTZ i
+| (HLEA.r r) := (EA.r r).read k sz w
+| (HLEA.m i a) :=
+  let n := sz.to_nat / 8 in
+  ∃ c v,
+    H.mem.nth i = some c ∧
+    c.2.1.to_nat + n ≤ c.2.2 ∧
+    k.mem.read (c.2.1 + a) v ∧
+    bits_to_byte n w v
+| (HLEA.abs _) := false -- absolute addresses are not for reading
+
+theorem HLEA.to_ea.read {H ea ea' k sz w}
+  (h1 : HLEA.to_ea H ea ea')
+  (h2 : ea.read H k sz w) : ea'.read k sz w :=
+begin
+  cases ea,
+  { cases h1, exact h2 },
+  { cases h1, exact h2 },
+  { rcases h1 with ⟨c, h1, rfl⟩,
+    rcases h2 with ⟨c', v', h1', e2, h2⟩, cases h1.symm.trans h1',
+    exact ⟨_, h2⟩ },
+  { cases h2 }
+end
+
+theorem HLEA.read.determ {H ea k sz w1 w2} :
+  HLEA.read H k sz w1 ea → ea.read H k sz w2 → w1 = w2 :=
+begin
+  cases ea,
+  { rintro ⟨⟩ ⟨⟩, refl },
+  { exact λ h1, h1.determ },
+  { rintro ⟨c1, v1, a1, b1, d1, e1⟩ ⟨c2, v2, a2, b2, d2, e2⟩,
+    cases a1.symm.trans a2,
+    cases d1.determ_len d2 (e1.1.trans e2.1.symm),
+    exact bits_to_byte.determ_l e1 e2 },
+  { rintro ⟨⟩ }
+end
+
+def HLEA.readq (H : hla) (k : config) (ea : HLEA) (sz : wsize) (q : qword) : Prop :=
+∃ w, ea.read H k sz w ∧ q = EXTZ w
+
+theorem HLEA.to_ea.readq {H ea ea' k sz w}
+  (h : HLEA.to_ea H ea ea') : ea.readq H k sz w → ea'.readq k sz w
+| ⟨w, h1, h2⟩ := ⟨_, h.read h1, h2⟩
+
+theorem HLEA.readq.determ {H ea k sz w1 w2} :
+  HLEA.readq H k ea sz w1 → ea.readq H k sz w2 → w1 = w2
+| ⟨w, h1, e1⟩ ⟨w2, h2, e2⟩ :=
+  by cases h1.determ h2; exact e1.trans e2.symm
+
+def HLEA.read' (H : hla) (ea : HLEA) (sz : wsize) : pstate config qword :=
+pstate.assert $ λ k, ea.readq H k sz
+
+def arg.read (H : hla) (k : config) (a : arg) (sz : wsize) (w : bitvec sz.to_nat) : Prop :=
+∃ ea, arg.ea H k a ea ∧ ea.read H k sz w
+
+def arg.readq (H : hla) (k : config) (a : arg) (sz : wsize) (q : qword) : Prop :=
+∃ ea, arg.ea H k a ea ∧ ea.readq H k sz q
+
+def arg.read' (H : hla) (a : arg) (sz : wsize) : pstate config qword :=
+pstate.assert $ λ k, a.readq H k sz
+
+def HLEA.write (H : hla) (k : config) (sz : wsize) (w : bitvec sz.to_nat) (k' : config) : HLEA → Prop
+| (HLEA.r r) := k' = config.write_reg k r sz w
+| (HLEA.m i a) :=
+  let n := sz.to_nat / 8 in
+  ∃ q m v,
+    H.mem.nth i = some (tt, (q, m)) ∧
+    q.to_nat + n ≤ m ∧
+    bits_to_byte n w v ∧
+    k.write_mem (q + a) v k'
+| _ := false
+
+def HLEA.writeq (H : hla) (k : config) (ea : HLEA) (sz : wsize) (q : qword) (k' : config) : Prop :=
+ea.write H k sz (EXTZ q) k'
+
+theorem HLEA.write.determ {H ea k sz w k1 k2} :
+  HLEA.write H k sz w k1 ea → ea.write H k sz w k2 → k1 = k2 :=
+begin
+  cases ea,
+  { rintro ⟨⟩ },
+  { rintro ⟨⟩ ⟨⟩, refl, },
+  { rintro ⟨q1, m1, v1, a1, b1, c1, d1⟩ ⟨q2, m2, v2, a2, b2, c2, d2⟩,
+    cases a1.symm.trans a2,
+    cases bits_to_byte.determ c1 c2,
+    exact d1.determ d2 },
+  { rintro ⟨⟩ },
+end
+
+theorem HLEA.writeq.determ {H ea k sz w k1 k2} :
+  HLEA.writeq H k ea sz w k1 → ea.writeq H k sz w k2 → k1 = k2 :=
+HLEA.write.determ
+
+theorem HLEA.to_ea.write {H ea ea' k k' sz w}
+  (h1 : HLEA.to_ea H ea ea')
+  (h2 : ea.write H k sz w k') : ea'.write k sz w k' :=
+begin
+  cases ea,
+  { cases h2 },
+  { cases h2, cases h1, constructor },
+  { rcases h2 with ⟨q, m, v, e1, e2, e3, e4⟩,
+    rcases h1 with ⟨c, e1', rfl⟩, cases e1.symm.trans e1',
+    exact EA.write.m e3 e4 },
+  { cases h2 }
+end
+
+theorem HLEA.to_ea.writeq {H ea ea' k k' sz w}
+  (h : HLEA.to_ea H ea ea') : ea.writeq H k sz w k' → ea'.writeq k sz w k' :=
+h.write
+
+def HLEA.write' (H : hla) (ea : HLEA) (sz : wsize) (q : qword) : pstate config unit :=
+pstate.lift $ λ k _ k', ea.writeq H k sz q k'
+
+def arg.writeq (H : hla) (k : config) (a : arg) (sz : wsize) (q : qword) (k' : config) : Prop :=
+∃ ea, arg.ea H k a ea ∧ ea.writeq H k sz q k'
+
+def arg.write' (H : hla) (a : arg) (sz : wsize) (q : qword) : pstate config unit :=
+pstate.lift $ λ k _ k', a.writeq H k sz q k'
+
+def asm1.exec (H : hla) : asm1 → pstate config unit
+| (asm1.unop op sz rm) := do
+  ea ← rm.ea' H,
+  w ← ea.read' H sz,
+  ea' ← ea.to_ea' H,
+  write_unop sz w ea' op
+| (asm1.binop op sz d s) := do
+  ea ← d.ea' H,
+  d' ← ea.read' H sz,
+  s' ← s.read' H sz,
+  ea' ← ea.to_ea' H,
+  write_binop sz ea' d' s' op
+| (asm1.mul sz r) := do
+  eax ← (EA.r RAX).read' sz,
+  src ← r.read' H sz,
+  execute._match_2 sz eax src sz,
+  erase_flags
+| (asm1.div sz r) := do
+  eax ← (EA.r RAX).read' sz,
+  edx ← (EA.r RDX).read' sz,
+  let n := edx.to_nat * (2 ^ sz.to_nat) + eax.to_nat,
+  d ← bitvec.to_nat <$> r.read' H sz,
+  pstate.assert $ λ _ (_:unit), d ≠ 0 ∧ n / d < 2 ^ sz.to_nat,
+  (EA.r RAX).write' sz (bitvec.of_nat _ (n / d)),
+  (EA.r RDX).write' sz (bitvec.of_nat _ (n % d)),
+  erase_flags
+| (asm1.lea sz d s) := do
+  src ← s.ea' H,
+  ea' ← src.to_ea' H,
+  d.write' H sz ea'.addr
+| (asm1.movsx sz1 d s sz2) := do
+  w ← pstate.assert $ λ k, s.read H k sz1,
+  d.write' H sz2 (EXTZ (EXTS w : bitvec sz2.to_nat))
+| (asm1.movzx sz1 d s sz2) := do
+  w ← pstate.assert $ λ k, s.read H k sz1,
+  d.write' H sz2 (EXTZ w)
+| (asm1.xchg sz r n) := do
+  let src := EA.r n,
+  dst ← r.ea' H,
+  val_src ← src.read' sz,
+  val_dst ← dst.read' H sz,
+  src.write' sz val_dst,
+  dst.write' H sz val_src
+| (asm1.cmpxchg sz r n) := do
+  let src := EA.r n,
+  let acc := EA.r RAX,
+  dst ← r.ea' H,
+  val_dst ← dst.read' H sz,
+  val_acc ← acc.read' sz,
+  write_binop sz src val_acc val_dst binop.cmp,
+  if val_acc = val_dst then
+    src.read' sz >>= dst.write' H sz
+  else acc.write' sz val_dst
+| (asm1.xadd sz r n) := do
+  let src := EA.r n,
+  dst ← r.ea' H >>= HLEA.to_ea' H,
+  val_src ← src.read' sz,
+  val_dst ← dst.read' sz,
+  src.write' sz val_dst,
+  write_binop sz dst val_src val_dst binop.add
+| (asm1.cmov c sz d s) := do
+  k ← pstate.get,
+  when (c.read k.flags) $ s.read' H sz >>= d.write' H sz
+| (asm1.setcc c b r) := do
+  k ← pstate.get,
+  r.write' H (wsize.Sz8 b) (EXTZ $ bitvec.singleton $ c.read k.flags)
+| (asm1.push i) := i.imm_rm' H >>= push
+| (asm1.pop r) := r.rm' H >>= pop
+| asm1.leave := do
+  (EA.r RBP).read' wsize.Sz64 >>= (EA.r RSP).write' wsize.Sz64,
+  pop (RM.reg RBP)
+| asm1.clc := write_flags $ λ _ f, {CF := ff, ..f}
+| asm1.cmc := write_flags $ λ _ f, {CF := bnot f.CF, ..f}
+| asm1.stc := write_flags $ λ _ f, {CF := tt, ..f}
+| asm1.syscall := pstate.fail
 
 def noIO_rel (P : config → config → Prop) : kcfg → kcfg → Prop
 | ⟨i, o, k⟩ ⟨i', o', k'⟩ := i = i' ∧ o = o' ∧ P k k'
 
-def asm1.kexec : kcfg → kcfg → asm1 → Prop
+def asm1.kexec (H : hla) : kcfg → kcfg → asm1 → Prop
 | ⟨i, o, k⟩ ⟨i', o', k'⟩ asm1.syscall := ∃ k1 k2 ret,
   config.isIO k k1 ∧
   exec_io i o k1 (k1.regs RAX) i' o' k2 ret →
   k' = k2.set_reg RAX ret
-| ⟨i, o, k⟩ ⟨i', o', k'⟩ a := i = i' ∧ o = o' ∧ a.exec k k'
+| ⟨i, o, k⟩ ⟨i', o', k'⟩ a := i = i' ∧ o = o' ∧ a.exec H k k'
 
 def asm1.pred (a : asm1) : code_pred :=
-λ _ _ _ v, ∃ a', a.pred' a' ∧ decode a' v
+λ H _ rip v, ∃ a', a.pred' H rip a' ∧ decode a' v
 
 def terminator.pred : terminator → code_pred
 | (terminator.jump a) H labs rip v := ∃ q,
@@ -333,7 +538,7 @@ def bblock.pred : bblock → code_pred
 structure kexit := (input output : list byte) (exit_code : qword)
 
 def bblock.kexec (H : hla) (labs : list qword) : bblock → kcfg → kcfg ⊕ kexit → Prop
-| (bblock.cons a b) k k' := ∃ k1, a.kexec k k1 ∧ b.kexec k1 k'
+| (bblock.cons a b) k k' := ∃ k1, a.kexec H k k1 ∧ b.kexec k1 k'
 | (bblock.term t) ⟨i, o, k⟩ (sum.inl ⟨i', o', k'⟩) :=
    i = i' ∧ o = o' ∧ t.exec H labs k (sum.inl k')
 | (bblock.term t) ⟨i, o, k⟩ (sum.inr ⟨i', o', c⟩) :=
@@ -356,142 +561,395 @@ def hla.blocks (H : hla) (l : list (list bblock)) : Prop :=
 ∀ i q n ll v, H.code.nth i = some ((q, n), (ll, v)) →
   ∃ bs, l.nth i = some bs ∧ bblocks.pred' H ll bs ll q v
 
-theorem asm1.exec_ok {a a'} (ha : asm1.pred' a a') {k k'} :
-  execute a' k k' ↔ a.exec k k' :=
+theorem asm1.exec_ok {H k a a'}
+  (ha : asm1.pred' H (k:config).rip a a') :
+  execute a' k ≤ a.exec H k :=
 begin
-  change (execute a' k).P () k' ↔ _,
   cases a,
   case hla.asm1.unop : op sz a {
     rcases ha with ⟨rm, h1, rfl⟩,
-    split,
-    { rintro ⟨_, _, ⟨⟩, q, _, ⟨h2, rfl⟩, h3⟩,
-      exact ⟨_, _, h1.ea, h2, h3⟩ },
-    { rintro ⟨ea, q, ⟨rm', h1', rfl⟩, h2, h3⟩,
-      cases (arg.rm_imm_rm.1 h1).determ h1',
-      exact ⟨_, _, ⟨_⟩, q, _, ⟨h2, rfl⟩, h3⟩ } },
+    rintro ⟨⟨_, _, h2, rfl⟩, R⟩,
+    rcases R _ _ ⟨h2, rfl⟩ with ⟨⟨_, _, h3, rfl⟩, R⟩,
+    rcases R _ _ ⟨h3, rfl⟩ with ⟨⟨_, _, h4, rfl⟩, R⟩,
+    refine ⟨⟨⟨_, _, ⟨_⟩⟩, _⟩, _⟩,
+    { rintro _ _ ⟨⟩,
+      have A := h1.ea h2,
+      have B := A.readq h3,
+      refine ⟨⟨_, _, B, rfl⟩, _⟩,
+      rintro _ _ ⟨h, rfl⟩, cases B.determ h,
+      exact R _ _ ⟨A, rfl⟩ },
+    { rintro _ _ ⟨_, _, ⟨⟩, _, _, ⟨B1, rfl⟩, B2⟩,
+      have A := h1.ea h2,
+      cases (A.readq h3).determ B1,
+      exact ⟨_, _, ⟨h2, rfl⟩, _, _, ⟨h3, rfl⟩, _, _, ⟨A, rfl⟩, B2⟩ } },
   case hla.asm1.binop : op sz d s {
     rcases ha with ⟨ds, h1, rfl⟩,
-    split,
-    { rintro ⟨⟨ea, d', s'⟩, _, ⟨⟨d, s, h2, h3⟩, rfl⟩, h4⟩,
-      exact ⟨_, _, _, h1.dest, h2, ⟨_, h1.src, h3⟩, h4⟩ },
-    { rintro ⟨_, d', s', hd, h3, ⟨s'', hs, _, h4, rfl⟩, h5⟩,
-      cases h1.dest.determ hd,
-      cases h1.src.determ hs,
-      exact ⟨⟨_, _, _⟩, _, ⟨⟨_, _, h3, _, h4, rfl⟩, rfl⟩, h5⟩ } },
+    rintro ⟨⟨dst, _, h2, rfl⟩, R⟩,
+    rcases R _ _ ⟨h2, rfl⟩ with ⟨⟨vd, _, h3, rfl⟩, R⟩,
+    rcases R _ _ ⟨h3, rfl⟩ with ⟨⟨vs, _, h4, rfl⟩, R⟩,
+    rcases R _ _ ⟨h4, rfl⟩ with ⟨⟨_, _, h5, rfl⟩, R⟩,
+    rcases id h4 with ⟨src, A1, A2⟩,
+    have A3 := h1.src A1,
+    cases h5.determ (h1.dest h2),
+    refine ⟨⟨⟨⟨_, _, _⟩, _,
+        ⟨_, _, h5.readq h3, (h1.src A1).readq A2⟩, rfl⟩, _⟩, _⟩,
+    { rintro ⟨_, _, _⟩ _ ⟨⟨_, _, B1, B2⟩, rfl⟩,
+      cases (h5.readq h3).determ B1,
+      cases (A3.readq A2).determ B2,
+      exact R _ _ ⟨h5, rfl⟩ },
+    { rintro _ _ ⟨⟨_, _, _⟩, _, ⟨⟨_, _, B1, B2⟩, rfl⟩, B3⟩,
+      cases (h5.readq h3).determ B1,
+      cases (A3.readq A2).determ B2,
+      refine ⟨_, _, ⟨h2, rfl⟩, _, _, ⟨h3, rfl⟩,
+        _, _, ⟨h4, rfl⟩, _, _, ⟨h5, rfl⟩, B3⟩ } },
   case hla.asm1.mul : sz a {
     rcases ha with ⟨rm, h1, rfl⟩,
-    split,
-    { rintro ⟨q, _, ⟨h2, rfl⟩, _, _, ⟨⟩,
-        q2, _, ⟨h3, rfl⟩, ⟨⟩, k1, h4, h5⟩,
-      refine ⟨_, _, _, h2, ⟨_, h1.ea, h3⟩, _, h5⟩,
-      cases sz, exact h4,
-      all_goals { rcases h4 with ⟨⟨⟩, k, h1, h2⟩, exact ⟨_, h1, h2⟩ } },
-    { rintro ⟨q, w, k1, h2, ⟨_, h1', h3⟩, h4, h5⟩,
-      cases h1.ea.determ h1',
-      refine ⟨_, _, ⟨h2, rfl⟩, _, _, ⟨_⟩, _, _, ⟨h3, rfl⟩, ⟨⟩, _, _, h5⟩,
-      cases sz, exact h4,
-      all_goals { rcases h4 with ⟨_, h1, h2⟩, exact ⟨⟨⟩, _, h1, h2⟩ } } },
+    rintro ⟨⟨rax, _, h2, rfl⟩, R⟩,
+    rcases R _ _ ⟨h2, rfl⟩ with ⟨⟨ad, _, h3, rfl⟩, R⟩,
+    rcases id h3 with ⟨ea, A1, A2⟩,
+    have A3 := (h1.ea A1).readq A2,
+    refine ⟨⟨⟨_, _, h2, rfl⟩, _⟩, _⟩,
+    { rintro _ _ ⟨B1, rfl⟩, cases h2.determ B1,
+      refine ⟨⟨_, _, ⟨_⟩⟩, _⟩, rintro _ _ ⟨⟩,
+      refine ⟨⟨_, _, ⟨A3, rfl⟩⟩, _⟩,
+      rintro _ _ ⟨B2, rfl⟩, cases A3.determ B2,
+      exact R _ _ ⟨h3, rfl⟩ },
+    { rintro _ _ ⟨_, _, ⟨B1, rfl⟩, _, _, ⟨⟩, _, _, ⟨B2, rfl⟩, B3⟩,
+      cases h2.determ B1, cases A3.determ B2,
+      exact ⟨_, _, ⟨h2, rfl⟩, _, _, ⟨h3, rfl⟩, B3⟩ } },
   case hla.asm1.div : sz a {
     rcases ha with ⟨rm, h1, rfl⟩,
-    split,
-    { rintro ⟨eax, _, ⟨h2, rfl⟩, edx, _, ⟨h3, rfl⟩, _, _, ⟨⟩, _, _,
-        ⟨d, _, ⟨h4, rfl⟩⟩, ⟨⟩, _, ⟨⟨h5, h6⟩, rfl⟩, ⟨⟩, _, h7, ⟨⟩, _, h8⟩,
-      exact ⟨_, _, _, _, _, h2, h3, ⟨_, h1.ea, h4⟩, h5, h6, h7, h8⟩ },
-    { rintro ⟨_, _, _, _, _, h2, h3, ⟨_, h1', h4⟩, h5, h6, h7, h8⟩,
-      cases h1.ea.determ h1',
-      exact ⟨_, _, ⟨h2, rfl⟩, _, _, ⟨h3, rfl⟩, _, _, ⟨_⟩, _, _,
-        ⟨_, _, _, ⟨h4, rfl⟩⟩, ⟨⟩, _, ⟨⟨h5, h6⟩, rfl⟩, ⟨⟩, _, h7, ⟨⟩, _, h8⟩ } },
+    rintro ⟨⟨rax, _, h2, rfl⟩, R⟩,
+    rcases R _ _ ⟨h2, rfl⟩ with ⟨⟨rdx, _, h3, rfl⟩, R⟩,
+    rcases R _ _ ⟨h3, rfl⟩ with ⟨⟨src, _, h4, rfl⟩, R⟩,
+    rcases R _ _ ⟨_, _, _, h4, rfl⟩ with ⟨⟨_, _, h5, rfl⟩, R⟩,
+    rcases id h4 with ⟨_, A1, A2⟩,
+    have A3 := (h1.ea A1).readq A2,
+    refine ⟨⟨⟨_, _, h2, rfl⟩, _⟩, _⟩,
+    { rintro _ _ ⟨B1, rfl⟩, cases h2.determ B1,
+      refine ⟨⟨_, _, ⟨h3, rfl⟩⟩, _⟩, rintro _ _ ⟨B2, rfl⟩, cases h3.determ B2,
+      refine ⟨⟨_, _, ⟨_⟩⟩, _⟩, rintro _ _ ⟨⟩,
+      refine ⟨⟨_, _, ⟨A3, rfl⟩⟩, _⟩, rintro _ _ ⟨_, _, B3, rfl⟩, cases A3.determ B3,
+      refine ⟨⟨⟨⟩, _, ⟨h5, rfl⟩⟩, _⟩, rintro _ _ ⟨B4, rfl⟩,
+      exact R ⟨⟩ _ ⟨h5, rfl⟩ },
+    { rintro _ _ ⟨_, _, ⟨B1, rfl⟩, _, _, ⟨B2, rfl⟩, _, _, ⟨⟩,
+        _, _, ⟨_, _, B3, rfl⟩, ⟨⟩, _, ⟨B4, rfl⟩, B5⟩,
+      cases h2.determ B1, cases h3.determ B2, cases A3.determ B3,
+      exact ⟨_, _, ⟨h2, rfl⟩, _, _, ⟨h3, rfl⟩,
+        _, _, ⟨_, _, _, h4, rfl⟩, ⟨⟩, _, ⟨h5, rfl⟩, B5⟩ } },
   case hla.asm1.lea : sz d s {
     rcases ha with ⟨ds, h1, rfl⟩,
-    split,
-    { rintro ⟨_, _, ⟨⟩, h2⟩,
-      exact ⟨_, h1.src, _, h1.dest, h2⟩ },
-    { rintro ⟨_, hs, _, hd, h2⟩,
-      cases h1.dest.determ hd,
-      cases h1.src.determ hs,
-      exact ⟨_, _, ⟨_⟩, h2⟩ } },
+    rintro ⟨⟨ea, _, h2, rfl⟩, R⟩,
+    rcases R _ _ ⟨h2, rfl⟩ with ⟨⟨ea', _, h3, rfl⟩, R⟩,
+    rcases R _ _ ⟨h3, rfl⟩ with ⟨⟨⟩, _, dst, h4, h5⟩,
+    cases (h1.src h2).determ h3,
+    have A1 := h1.dest h4,
+    refine ⟨⟨⟨_, _, ⟨_⟩⟩, _⟩, _⟩,
+    { rintro _ _ ⟨⟩, exact ⟨⟨⟩, _, A1.writeq h5⟩ },
+    { rintro _ _ ⟨_, _, ⟨⟩, B1⟩,
+      cases (A1.writeq h5).determ B1,
+      refine ⟨_, _, ⟨h2, rfl⟩, _, _, ⟨h3, rfl⟩, _, h4, h5⟩ } },
   iterate 2 {
     rcases ha with ⟨ds, h1, rfl⟩,
-    split,
-    { rintro ⟨_, _, ⟨h2, rfl⟩, _, _, ⟨⟩, h3⟩,
-      exact ⟨_, ⟨_, h1.src, h2⟩, _, h1.dest, h3⟩ },
-    { rintro ⟨_, ⟨_, hs, h2⟩, _, hd, h3⟩,
-      cases h1.dest.determ hd,
-      cases h1.src.determ hs,
-      exact ⟨_, _, ⟨h2, rfl⟩, _, _, ⟨_⟩, h3⟩ } },
+    rintro ⟨⟨ea, _, h2, rfl⟩, R⟩,
+    rcases R _ _ ⟨h2, rfl⟩ with ⟨⟨⟩, _, h3⟩,
+    rcases id h2 with ⟨_, A1, A2⟩,
+    rcases id h3 with ⟨_, A3, A4⟩,
+    have A5 := (h1.src A1).read A2,
+    have A6 := (h1.dest A3).writeq A4,
+    refine ⟨⟨⟨_, _, A5, rfl⟩, _⟩, _⟩,
+    { rintro _ _ ⟨B1, rfl⟩, cases A5.determ B1,
+      refine ⟨⟨_, _, ⟨_⟩⟩, _⟩, rintro _ _ ⟨⟩,
+      refine ⟨⟨⟩, _, A6⟩ },
+    { rintro _ _ ⟨_, _, ⟨B1, rfl⟩, _, _, ⟨⟩, B2⟩,
+      cases A5.determ B1, cases A6.determ B2,
+      refine ⟨_, _, ⟨h2, rfl⟩, _, A3, A4⟩ } },
   case hla.asm1.xchg : sz a r {
     rcases ha with ⟨rm, h1, rfl⟩,
-    split,
-    { rintro ⟨_, _, ⟨⟩, _, _, ⟨h2, rfl⟩, _, _, ⟨h3, rfl⟩, ⟨⟩, _, h4⟩,
-      exact ⟨_, _, _, _, h1.ea, h2, h3, h4⟩ },
-    { rintro ⟨_, _, _, _, h1', h2, h3, h4⟩,
-      cases h1.ea.determ h1',
-      exact ⟨_, _, ⟨_⟩, _, _, ⟨h2, rfl⟩, _, _, ⟨h3, rfl⟩, ⟨⟩, _, h4⟩ } },
-  case hla.asm1.cmpxchg : sz a r {
-    rcases ha with ⟨rm, h1, rfl⟩,
-    split,
-    { rintro ⟨_, _, ⟨⟩, _, _, ⟨h2, rfl⟩, _, _, ⟨h3, rfl⟩, h4⟩,
-      exact ⟨_, _, _, h1.ea, h2, h3, h4⟩ },
-    { rintro ⟨_, _, _, h1', h2, h3, h4⟩,
-      cases h1.ea.determ h1',
-      exact ⟨_, _, ⟨_⟩, _, _, ⟨h2, rfl⟩, _, _, ⟨h3, rfl⟩, h4⟩ } },
-  case hla.asm1.xadd : sz a r {
-    rcases ha with ⟨rm, h1, rfl⟩,
-    split,
-    { rintro ⟨_, _, ⟨⟩, _, _, ⟨h2, rfl⟩, _, _, ⟨h3, rfl⟩, ⟨⟩, _, h4⟩,
-      exact ⟨_, _, _, _, h1.ea, h2, h3, h4⟩ },
-    { rintro ⟨_, _, _, _, h1', h2, h3, h4⟩,
-      cases h1.ea.determ h1',
-      exact ⟨_, _, ⟨_⟩, _, _, ⟨h2, rfl⟩, _, _, ⟨h3, rfl⟩, ⟨⟩, _, h4⟩, } },
-  case hla.asm1.cmov : c sz d s {
-    rcases ha with ⟨ds, h1, rfl⟩,
-    change _ ↔ cond _ _ _,
-    split,
-    { rintro ⟨_, _, ⟨⟩, h2⟩, dsimp only at h2,
-      revert h2, cases c.read k.flags,
-      { rintro ⟨⟩, exact rfl },
-      { rintro ⟨_, _, ⟨h3, rfl⟩, h4⟩,
-        exact ⟨_, ⟨_, h1.src, h3⟩, _, h1.dest, h4⟩ } },
-    { intro h2, refine ⟨_, _, ⟨_⟩, _⟩, dsimp only,
-      revert h2, cases c.read k.flags,
-      { rintro ⟨⟩, exact ⟨_, _⟩ },
-      { rintro ⟨_, ⟨_, hs, h3⟩, _, hd, h4⟩,
-        cases h1.dest.determ hd,
-        cases h1.src.determ hs,
-        exact ⟨_, _, ⟨h3, rfl⟩, h4⟩ } } },
-  case hla.asm1.setcc : c b a {
-    rcases ha with ⟨rm, h1, rfl⟩,
-    split,
-    { rintro ⟨_, _, ⟨⟩, h2⟩,
-      exact ⟨_, h1.ea, h2⟩ },
-    { rintro ⟨_, h1', h2⟩,
-      cases h1.ea.determ h1',
-      exact ⟨_, _, ⟨_⟩, h2⟩ } },
-  iterate 2 {
-    rcases ha with ⟨rm, h1, rfl⟩,
-    split,
-    { exact λ h2, ⟨_, h1, h2⟩ },
-    { rintro ⟨_, h1', h2⟩,
-      cases h1.determ h1',
-      exact h2 } },
-  case hla.asm1.leave {
-    cases ha, split,
-    { rintro ⟨_, _, ⟨_, _, ⟨h2, rfl⟩, h3⟩, h4⟩,
-      cases EA.readq_reg_64.1 h2,
-      cases EA.writeq_reg_64.1 h3,
-      exact h4 },
-    { rintro h4,
-      exact ⟨⟨⟩, _, ⟨_, _,
-        ⟨EA.readq_reg_64.2 rfl, rfl⟩, EA.writeq_reg_64.2 rfl⟩, h4⟩ } },
-  iterate 3 {
-    cases ha, split,
-    { rintro ⟨⟩, constructor },
-    { rintro ⟨⟩, constructor } },
-  case hla.asm1.syscall { cases ha, split; rintro ⟨⟨⟩⟩ },
+    rintro ⟨⟨ea, _, h2, rfl⟩, R⟩,
+    rcases R _ _ ⟨h2, rfl⟩ with ⟨⟨dst, _, h3, rfl⟩, R⟩,
+    rcases R _ _ ⟨h3, rfl⟩ with ⟨⟨vs, _, h4, rfl⟩, R⟩,
+    rcases R _ _ ⟨h4, rfl⟩ with ⟨⟨⟨⟩, _, h5⟩, R⟩,
+    sorry, },
+    -- cases (h1.src h2).determ h3,
+    -- have A1 := h1.dest h4,
+    -- refine ⟨⟨⟨_, _, ⟨_⟩⟩, _⟩, _⟩,
+    -- { rintro _ _ ⟨⟩, exact ⟨⟨⟩, _, A1.writeq h5⟩ },
+    -- { rintro _ _ ⟨_, _, ⟨⟩, B1⟩,
+    --   cases (A1.writeq h5).determ B1,
+    --   refine ⟨_, _, ⟨h2, rfl⟩, _, _, ⟨h3, rfl⟩, _, h4, h5⟩ } },
+    -- split,
+    -- { rintro ⟨_, _, ⟨⟩, _, _, ⟨h2, rfl⟩, _, _, ⟨h3, rfl⟩, ⟨⟩, _, h4⟩,
+    --   exact ⟨_, _, _, _, h1.ea, h2, h3, h4⟩ },
+    -- { rintro ⟨_, _, _, _, h1', h2, h3, h4⟩,
+    --   cases h1.ea.determ h1',
+    --   exact ⟨_, _, ⟨_⟩, _, _, ⟨h2, rfl⟩, _, _, ⟨h3, rfl⟩, ⟨⟩, _, h4⟩ } },
+  -- case hla.asm1.cmpxchg : sz a r {
+  --   rcases ha with ⟨rm, h1, rfl⟩,
+  --   split,
+  --   { rintro ⟨_, _, ⟨⟩, _, _, ⟨h2, rfl⟩, _, _, ⟨h3, rfl⟩, h4⟩,
+  --     exact ⟨_, _, _, h1.ea, h2, h3, h4⟩ },
+  --   { rintro ⟨_, _, _, h1', h2, h3, h4⟩,
+  --     cases h1.ea.determ h1',
+  --     exact ⟨_, _, ⟨_⟩, _, _, ⟨h2, rfl⟩, _, _, ⟨h3, rfl⟩, h4⟩ } },
+  -- case hla.asm1.xadd : sz a r {
+  --   rcases ha with ⟨rm, h1, rfl⟩,
+  --   split,
+  --   { rintro ⟨_, _, ⟨⟩, _, _, ⟨h2, rfl⟩, _, _, ⟨h3, rfl⟩, ⟨⟩, _, h4⟩,
+  --     exact ⟨_, _, _, _, h1.ea, h2, h3, h4⟩ },
+  --   { rintro ⟨_, _, _, _, h1', h2, h3, h4⟩,
+  --     cases h1.ea.determ h1',
+  --     exact ⟨_, _, ⟨_⟩, _, _, ⟨h2, rfl⟩, _, _, ⟨h3, rfl⟩, ⟨⟩, _, h4⟩, } },
+  -- case hla.asm1.cmov : c sz d s {
+  --   rcases ha with ⟨ds, h1, rfl⟩,
+  --   change _ ↔ cond _ _ _,
+  --   split,
+  --   { rintro ⟨_, _, ⟨⟩, h2⟩, dsimp only at h2,
+  --     revert h2, cases c.read k.flags,
+  --     { rintro ⟨⟩, exact rfl },
+  --     { rintro ⟨_, _, ⟨h3, rfl⟩, h4⟩,
+  --       exact ⟨_, ⟨_, h1.src, h3⟩, _, h1.dest, h4⟩ } },
+  --   { intro h2, refine ⟨_, _, ⟨_⟩, _⟩, dsimp only,
+  --     revert h2, cases c.read k.flags,
+  --     { rintro ⟨⟩, exact ⟨_, _⟩ },
+  --     { rintro ⟨_, ⟨_, hs, h3⟩, _, hd, h4⟩,
+  --       cases h1.dest.determ hd,
+  --       cases h1.src.determ hs,
+  --       exact ⟨_, _, ⟨h3, rfl⟩, h4⟩ } } },
+  -- case hla.asm1.setcc : c b a {
+  --   rcases ha with ⟨rm, h1, rfl⟩,
+  --   split,
+  --   { rintro ⟨_, _, ⟨⟩, h2⟩,
+  --     exact ⟨_, h1.ea, h2⟩ },
+  --   { rintro ⟨_, h1', h2⟩,
+  --     cases h1.ea.determ h1',
+  --     exact ⟨_, _, ⟨_⟩, h2⟩ } },
+  -- iterate 2 {
+  --   rcases ha with ⟨rm, h1, rfl⟩,
+  --   split,
+  --   { exact λ h2, ⟨_, h1, h2⟩ },
+  --   { rintro ⟨_, h1', h2⟩,
+  --     cases h1.determ h1',
+  --     exact h2 } },
+  -- case hla.asm1.leave {
+  --   cases ha, split,
+  --   { rintro ⟨_, _, ⟨_, _, ⟨h2, rfl⟩, h3⟩, h4⟩,
+  --     cases EA.readq_reg_64.1 h2,
+  --     cases EA.writeq_reg_64.1 h3,
+  --     exact h4 },
+  --   { rintro h4,
+  --     exact ⟨⟨⟩, _, ⟨_, _,
+  --       ⟨EA.readq_reg_64.2 rfl, rfl⟩, EA.writeq_reg_64.2 rfl⟩, h4⟩ } },
+  -- iterate 3 {
+  --   cases ha, split,
+  --   { rintro ⟨⟩, constructor },
+  --   { rintro ⟨⟩, constructor } },
+  -- case hla.asm1.syscall { cases ha, split; rintro ⟨⟨⟩⟩ },
+
+  -- case hla.asm1.unop : op sz a {
+  --   rcases ha with ⟨rm, h1, rfl⟩,
+  --   split,
+  --   { rintro ⟨_, _, ⟨⟩, q, _, ⟨h2, rfl⟩, h3⟩,
+  --     exact ⟨_, _, h1.ea, h2, h3⟩ },
+  --   { rintro ⟨ea, q, ⟨rm', h1', rfl⟩, h2, h3⟩,
+  --     cases (arg.rm_imm_rm.1 h1).determ h1',
+  --     exact ⟨_, _, ⟨_⟩, q, _, ⟨h2, rfl⟩, h3⟩ } },
+  -- case hla.asm1.binop : op sz d s {
+  --   rcases ha with ⟨ds, h1, rfl⟩,
+  --   split,
+  --   { rintro ⟨⟨ea, d', s'⟩, _, ⟨⟨d, s, h2, h3⟩, rfl⟩, h4⟩,
+  --     exact ⟨_, _, _, h1.dest, h2, ⟨_, h1.src, h3⟩, h4⟩ },
+  --   { rintro ⟨_, d', s', hd, h3, ⟨s'', hs, _, h4, rfl⟩, h5⟩,
+  --     cases h1.dest.determ hd,
+  --     cases h1.src.determ hs,
+  --     exact ⟨⟨_, _, _⟩, _, ⟨⟨_, _, h3, _, h4, rfl⟩, rfl⟩, h5⟩ } },
+  -- case hla.asm1.mul : sz a {
+  --   rcases ha with ⟨rm, h1, rfl⟩,
+  --   split,
+  --   { rintro ⟨q, _, ⟨h2, rfl⟩, _, _, ⟨⟩,
+  --       q2, _, ⟨h3, rfl⟩, ⟨⟩, k1, h4, h5⟩,
+  --     refine ⟨_, _, _, h2, ⟨_, h1.ea, h3⟩, _, h5⟩,
+  --     cases sz, exact h4,
+  --     all_goals { rcases h4 with ⟨⟨⟩, k, h1, h2⟩, exact ⟨_, h1, h2⟩ } },
+  --   { rintro ⟨q, w, k1, h2, ⟨_, h1', h3⟩, h4, h5⟩,
+  --     cases h1.ea.determ h1',
+  --     refine ⟨_, _, ⟨h2, rfl⟩, _, _, ⟨_⟩, _, _, ⟨h3, rfl⟩, ⟨⟩, _, _, h5⟩,
+  --     cases sz, exact h4,
+  --     all_goals { rcases h4 with ⟨_, h1, h2⟩, exact ⟨⟨⟩, _, h1, h2⟩ } } },
+  -- case hla.asm1.div : sz a {
+  --   rcases ha with ⟨rm, h1, rfl⟩,
+  --   split,
+  --   { rintro ⟨eax, _, ⟨h2, rfl⟩, edx, _, ⟨h3, rfl⟩, _, _, ⟨⟩, _, _,
+  --       ⟨d, _, ⟨h4, rfl⟩⟩, ⟨⟩, _, ⟨⟨h5, h6⟩, rfl⟩, ⟨⟩, _, h7, ⟨⟩, _, h8⟩,
+  --     exact ⟨_, _, _, _, _, h2, h3, ⟨_, h1.ea, h4⟩, h5, h6, h7, h8⟩ },
+  --   { rintro ⟨_, _, _, _, _, h2, h3, ⟨_, h1', h4⟩, h5, h6, h7, h8⟩,
+  --     cases h1.ea.determ h1',
+  --     exact ⟨_, _, ⟨h2, rfl⟩, _, _, ⟨h3, rfl⟩, _, _, ⟨_⟩, _, _,
+  --       ⟨_, _, _, ⟨h4, rfl⟩⟩, ⟨⟩, _, ⟨⟨h5, h6⟩, rfl⟩, ⟨⟩, _, h7, ⟨⟩, _, h8⟩ } },
+  -- case hla.asm1.lea : sz d s {
+  --   rcases ha with ⟨ds, h1, rfl⟩,
+  --   split,
+  --   { rintro ⟨_, _, ⟨⟩, h2⟩,
+  --     exact ⟨_, h1.src, _, h1.dest, h2⟩ },
+  --   { rintro ⟨_, hs, _, hd, h2⟩,
+  --     cases h1.dest.determ hd,
+  --     cases h1.src.determ hs,
+  --     exact ⟨_, _, ⟨_⟩, h2⟩ } },
+  -- iterate 2 {
+  --   rcases ha with ⟨ds, h1, rfl⟩,
+  --   split,
+  --   { rintro ⟨_, _, ⟨h2, rfl⟩, _, _, ⟨⟩, h3⟩,
+  --     exact ⟨_, ⟨_, h1.src, h2⟩, _, h1.dest, h3⟩ },
+  --   { rintro ⟨_, ⟨_, hs, h2⟩, _, hd, h3⟩,
+  --     cases h1.dest.determ hd,
+  --     cases h1.src.determ hs,
+  --     exact ⟨_, _, ⟨h2, rfl⟩, _, _, ⟨_⟩, h3⟩ } },
+  -- case hla.asm1.xchg : sz a r {
+  --   rcases ha with ⟨rm, h1, rfl⟩,
+  --   split,
+  --   { rintro ⟨_, _, ⟨⟩, _, _, ⟨h2, rfl⟩, _, _, ⟨h3, rfl⟩, ⟨⟩, _, h4⟩,
+  --     exact ⟨_, _, _, _, h1.ea, h2, h3, h4⟩ },
+  --   { rintro ⟨_, _, _, _, h1', h2, h3, h4⟩,
+  --     cases h1.ea.determ h1',
+  --     exact ⟨_, _, ⟨_⟩, _, _, ⟨h2, rfl⟩, _, _, ⟨h3, rfl⟩, ⟨⟩, _, h4⟩ } },
+  -- case hla.asm1.cmpxchg : sz a r {
+  --   rcases ha with ⟨rm, h1, rfl⟩,
+  --   split,
+  --   { rintro ⟨_, _, ⟨⟩, _, _, ⟨h2, rfl⟩, _, _, ⟨h3, rfl⟩, h4⟩,
+  --     exact ⟨_, _, _, h1.ea, h2, h3, h4⟩ },
+  --   { rintro ⟨_, _, _, h1', h2, h3, h4⟩,
+  --     cases h1.ea.determ h1',
+  --     exact ⟨_, _, ⟨_⟩, _, _, ⟨h2, rfl⟩, _, _, ⟨h3, rfl⟩, h4⟩ } },
+  -- case hla.asm1.xadd : sz a r {
+  --   rcases ha with ⟨rm, h1, rfl⟩,
+  --   split,
+  --   { rintro ⟨_, _, ⟨⟩, _, _, ⟨h2, rfl⟩, _, _, ⟨h3, rfl⟩, ⟨⟩, _, h4⟩,
+  --     exact ⟨_, _, _, _, h1.ea, h2, h3, h4⟩ },
+  --   { rintro ⟨_, _, _, _, h1', h2, h3, h4⟩,
+  --     cases h1.ea.determ h1',
+  --     exact ⟨_, _, ⟨_⟩, _, _, ⟨h2, rfl⟩, _, _, ⟨h3, rfl⟩, ⟨⟩, _, h4⟩, } },
+  -- case hla.asm1.cmov : c sz d s {
+  --   rcases ha with ⟨ds, h1, rfl⟩,
+  --   change _ ↔ cond _ _ _,
+  --   split,
+  --   { rintro ⟨_, _, ⟨⟩, h2⟩, dsimp only at h2,
+  --     revert h2, cases c.read k.flags,
+  --     { rintro ⟨⟩, exact rfl },
+  --     { rintro ⟨_, _, ⟨h3, rfl⟩, h4⟩,
+  --       exact ⟨_, ⟨_, h1.src, h3⟩, _, h1.dest, h4⟩ } },
+  --   { intro h2, refine ⟨_, _, ⟨_⟩, _⟩, dsimp only,
+  --     revert h2, cases c.read k.flags,
+  --     { rintro ⟨⟩, exact ⟨_, _⟩ },
+  --     { rintro ⟨_, ⟨_, hs, h3⟩, _, hd, h4⟩,
+  --       cases h1.dest.determ hd,
+  --       cases h1.src.determ hs,
+  --       exact ⟨_, _, ⟨h3, rfl⟩, h4⟩ } } },
+  -- case hla.asm1.setcc : c b a {
+  --   rcases ha with ⟨rm, h1, rfl⟩,
+  --   split,
+  --   { rintro ⟨_, _, ⟨⟩, h2⟩,
+  --     exact ⟨_, h1.ea, h2⟩ },
+  --   { rintro ⟨_, h1', h2⟩,
+  --     cases h1.ea.determ h1',
+  --     exact ⟨_, _, ⟨_⟩, h2⟩ } },
+  -- iterate 2 {
+  --   rcases ha with ⟨rm, h1, rfl⟩,
+  --   split,
+  --   { exact λ h2, ⟨_, h1, h2⟩ },
+  --   { rintro ⟨_, h1', h2⟩,
+  --     cases h1.determ h1',
+  --     exact h2 } },
+  -- case hla.asm1.leave {
+  --   cases ha, split,
+  --   { rintro ⟨_, _, ⟨_, _, ⟨h2, rfl⟩, h3⟩, h4⟩,
+  --     cases EA.readq_reg_64.1 h2,
+  --     cases EA.writeq_reg_64.1 h3,
+  --     exact h4 },
+  --   { rintro h4,
+  --     exact ⟨⟨⟩, _, ⟨_, _,
+  --       ⟨EA.readq_reg_64.2 rfl, rfl⟩, EA.writeq_reg_64.2 rfl⟩, h4⟩ } },
+  -- iterate 3 {
+  --   cases ha, split,
+  --   { rintro ⟨⟩, constructor },
+  --   { rintro ⟨⟩, constructor } },
+  -- case hla.asm1.syscall { cases ha, split; rintro ⟨⟨⟩⟩ },
+  repeat {sorry}
 end
+
+theorem terminator.exec_ok {H labs rip t v}
+  (ha : terminator.pred t H labs rip v) {k k'} :
+  execute a' k k' ↔ a.exec k k' :=
 
 theorem code_pred.cons_ok {a b H k labs}
   (h : (code_pred.cons a b).ok H k labs) : a.ok H k labs := sorry
+
+def hla_ok {α} (F : pstate config α) : Prop :=
+∀ {{H : hla}} {{a k k'}}, (F k).P a k' → H.ok k → H.ok k'
+
+theorem hla_ok.pure {α} {a : α} : hla_ok (pure a) :=
+by rintro H a k k' ⟨⟩; exact id
+
+theorem hla_ok.return {α} {a : α} : hla_ok (return a) :=
+hla_ok.pure
+
+theorem hla_ok.bind {α β} {m : pstate config α} {f : α → pstate config β}
+  (H1 : hla_ok m) (H2 : ∀ b, hla_ok (f b)) :
+  hla_ok (m >>= f) :=
+by rintro H a k k' ⟨a, k1, h1, h2⟩ h; exact H2 _ h2 (H1 h1 h)
+
+theorem hla_ok.map {α β} {m : pstate config α} {f : α → β}
+  (H1 : hla_ok m) : hla_ok (f <$> m) :=
+by rintro H a k k' ⟨a, h1, h2⟩; exact H1 h2
+
+theorem hla_ok.lift {α} {f : config → α → config → Prop}
+  (H : ∀ {{H : hla}} {{a k k'}}, f k a k' → H.ok k → H.ok k') :
+  hla_ok (pstate.lift f) := H
+
+theorem hla_ok.get : hla_ok pstate.get :=
+by rintro H a k k' ⟨⟩; exact id
+
+theorem hla_ok.assert {α} {p : config → α → Prop} :
+  hla_ok (pstate.assert p) :=
+by rintro H a k k' ⟨_, rfl⟩; exact id
+
+theorem hla_ok.modify {f : config → config}
+  (h : ∀ {{H : hla}} {{k}}, H.ok k → H.ok (f k)) :
+  hla_ok (pstate.modify f) :=
+by rintro H _ k k' ⟨_, rfl⟩; apply h
+
+theorem hla_ok.any {α} {p : config → α → Prop} :
+  hla_ok (@pstate.any _ α) :=
+hla_ok.assert
+
+theorem hla_ok.fail {α} {p : config → α → Prop} :
+  hla_ok (@pstate.fail _ α) :=
+hla_ok.assert
+
+theorem hla_ok_mem_read {H : hla} {k k' : config}
+  (h1 : ∀ p q v, k.mem.read' p q v →
+    ∃ v', list.length v' = v.length ∧ k'.mem.read' p q v') :
+  H.ok k → H.ok k'
+| ⟨h2, h3⟩ := begin
+  refine ⟨λ b q n m, _, λ q n ll v m, _⟩,
+  { rcases h2 b q n m with ⟨v1, rfl, h4⟩,
+    exact h1 _ _ _ h4 },
+  { rcases h2 b q n m with ⟨v1, rfl, h4⟩,
+    have := h3 q n ll v' m,
+  }
+end
+
+theorem hla_ok_mem_eq {H : hla} {k k' : config}
+  (e : k.mem = k'.mem) (h : H.ok k) : H.ok k' :=
+_
+
+theorem hla_ok.write_rip {q} : hla_ok (write_rip q) :=
+hla_ok.modify $ λ H k, _
+
+theorem hla.ok.step {H : hla} {k k' : config}
+  (hk : H.ok k) (h : k.step k') : H.ok k' :=
+begin
+  cases h with _ _ _ _ _ h,
+end
 
 theorem bblock.exec_cons (H : hla) {k k' : config} (hk : H.ok k)
   {l} (hl : H.blocks l)
