mm0-lean/x86/lemmas.lean
@@ -55,7 +55,7 @@ begin
   exact congr_arg (vector.cons l_hd) (n_ih _ h_1)
 end
 
-theorem of_nat_to_nat : ∀ {n} (v : bitvec n),
+@[simp] theorem of_nat_to_nat : ∀ {n} (v : bitvec n),
   bitvec.of_nat n (to_nat v) = v
 | n ⟨l, e⟩ := of_nat_bits_to_nat_eq l e
 
@@ -99,7 +99,7 @@ theorem of_zmod_to_zmod {n} (v : bitvec n) : of_zmod (to_zmod v) = v :=
 by unfold of_zmod to_zmod; convert of_nat_to_nat v; exact
 zmod.val_cast_of_lt (to_nat_lt_pow2 _)
 
-theorem to_nat_eq_iff_modeq {m n₁ n₂} :
+theorem of_nat_eq_iff_modeq {m n₁ n₂} :
   bitvec.of_nat m n₁ = bitvec.of_nat m n₂ ↔ n₁ ≡ n₂ [MOD 2 ^ m] :=
 begin
   dunfold nat.modeq, split; intro h,
@@ -110,7 +110,7 @@ end
 
 theorem of_nat_eq_of_zmod (m n) :
   bitvec.of_nat m n = bitvec.of_zmod n :=
-eq.symm $ to_nat_eq_iff_modeq.2 $
+eq.symm $ of_nat_eq_iff_modeq.2 $
 by convert nat.modeq.mod_modeq _ _; apply zmod.val_cast_nat
 
 theorem to_zmod_zero (n) : to_zmod (0 : bitvec n) = 0 :=
@@ -254,6 +254,25 @@ theorem add_nat_assoc {n} (v : bitvec n) (a b : ℕ) :
   v + a + b = v + (a + b : ℕ) :=
 by rw [nat.cast_add, add_assoc]
 
+theorem of_nat_add {n} (a b : ℕ) : bitvec.of_nat n (a + b) = bitvec.of_nat n a + bitvec.of_nat n b :=
+by simp [of_nat_eq_of_zmod, of_zmod_add]
+
+theorem of_nat_succ' {n} (a : ℕ) : bitvec.of_nat n a.succ = bitvec.of_nat n a + 1 :=
+(of_nat_add a 1).trans $ by simp [of_nat_one]
+
+theorem of_nat_mul {n} (a b : ℕ) : bitvec.of_nat n (a * b) = bitvec.of_nat n a * bitvec.of_nat n b :=
+by simp [of_nat_eq_of_zmod, of_zmod_mul]
+
+theorem coe_eq_of_nat {n} (a : ℕ) :
+  (a : bitvec n) = bitvec.of_nat n a :=
+begin
+  induction a, exact (bitvec.of_nat_zero _).symm,
+  rw [of_nat_succ', ← a_ih], refl,
+end
+
+theorem coe_to_nat {n} (v : bitvec n) : (to_nat v : bitvec n) = v :=
+by rw [coe_eq_of_nat, of_nat_to_nat]
+
 theorem bits_to_nat_inj : ∀ {l₁ l₂},
   bits_to_nat l₁ = bits_to_nat l₂ → l₁.length = l₂.length → l₁ = l₂
 | [] [] _ _ := rfl
@@ -268,12 +287,18 @@ theorem to_nat_inj {n v₁ v₂}
   (h : @bitvec.to_nat n v₁ = bitvec.to_nat v₂) : v₁ = v₂ :=
 subtype.eq $ bits_to_nat_inj h (v₁.2.trans v₂.2.symm)
 
+theorem coe_shl {n} (a b) : (nat.shiftl a b : bitvec n) = bitvec.shl a b :=
+begin
+  rw [shl, coe_eq_of_nat, nat.shiftl_eq_mul_pow, nat.shiftl_eq_mul_pow],
+  refine of_nat_eq_iff_modeq.2 (nat.modeq.modeq_mul_right _ _),
+  rw [← of_nat_eq_iff_modeq, of_nat_to_nat, coe_eq_of_nat],
+end
+
 theorem sign_iff_neg {n v} : @bitvec.sign n v ↔ bitvec.to_int v < 0 :=
 begin
   unfold bitvec.to_int, cases sign v; simp,
   apply sub_lt_zero.2, norm_cast,
-  exact lt_trans (to_nat_lt_pow2 _)
-    (nat.pow_lt_pow_of_lt_right dec_trivial (nat.lt_succ_self _)),
+  exact to_nat_lt_pow2 _
 end
 
 theorem to_int_inj {n v₁ v₂}
@@ -286,6 +311,17 @@ begin
   unfold bitvec.to_int,
   rw this, cases sign v₂; simp; exact to_nat_inj
 end
+
+theorem pow2_eq_zero {n} : (2 ^ n : bitvec n) = 0 :=
+begin
+  suffices : ((2 ^ n : ℕ) : bitvec n) = 0, {exact_mod_cast this},
+  have := to_nat_of_nat n (2^n),
+  apply to_nat_inj,
+  rw [coe_eq_of_nat, to_nat_of_nat, nat.mod_self, to_nat_zero],
+end
+
+theorem coe_to_int {n} (v : bitvec n) : (to_int v : bitvec n) = v :=
+by unfold to_int; cases sign v; simp [coe_to_nat, pow2_eq_zero]
 
 @[class] def reify {n} (v : bitvec n) (l : out_param (list bool)) : Prop :=
 from_bits_fill ff l = v
@@ -1340,9 +1376,9 @@ theorem mem.read1.determ {p1 p2 m a b1 b2} :
   mem.read1 p1 m a b1 → mem.read1 p2 m a b2 → b1 = b2 :=
 by rintro ⟨_, rfl, _⟩ ⟨_, rfl, _⟩; refl
 
-theorem mem.read.determ_aux {p1 p2 m a l1 l2}
+theorem mem.read'.determ_aux {p1 p2 m a l1 l2}
   (h₁ : mem.read' p1 m a l1) (h₂ : mem.read' p2 m a l2) :
-   l1 <+: l2 ∨ l2 <+: l1 :=
+  l1 <+: l2 ∨ l2 <+: l1 :=
 begin
   induction h₁ generalizing l2,
   { exact or.inl (list.nil_prefix _) },
@@ -1353,12 +1389,19 @@ begin
   exact h₁_ih h₂_a_1,
 end
 
+theorem mem.read'.determ_len {p1 p2 m a l1 l2}
+  (h₁ : mem.read' p1 m a l1) (h₂ : mem.read' p2 m a l2)
+  (h : l1.length = l2.length) : l1 = l2 :=
+(mem.read'.determ_aux h₁ h₂).elim
+  (λ h', list.eq_of_prefix_of_length_eq h' h)
+  (λ h', (list.eq_of_prefix_of_length_eq h' h.symm).symm)
+
 theorem mem_decode.determ {p1 p2 m a l1 l2 ast1 ast2}
   (m₁ :  mem.read' p1 m a l1) (h₁ : decode ast1 l1)
   (m₂ :  mem.read' p2 m a l2) (h₂ : decode ast2 l2) :
   (ast1, l1) = (ast2, l2) :=
 begin
-  rcases mem.read.determ_aux m₁ m₂ with ⟨x, rfl⟩ | ⟨x, rfl⟩,
+  rcases mem.read'.determ_aux m₁ m₂ with ⟨x, rfl⟩ | ⟨x, rfl⟩,
   { cases decode.determ_aux h₁ h₂, simp },
   { cases decode.determ_aux h₂ h₁, simp },
 end
@@ -1501,19 +1544,73 @@ begin
 end
 
 theorem EA.read_reg_64 {r k q} :
-  (EA.EA_r r).read k wsize.Sz64 q ↔ q = k.regs r :=
+  (EA.r r).read k wsize.Sz64 q ↔ q = k.regs r :=
 by simp [EA.read]
 
 theorem EA.readq_reg_64 {r k q} :
-  (EA.EA_r r).readq k wsize.Sz64 q ↔ q = k.regs r :=
+  (EA.r r).readq k wsize.Sz64 q ↔ q = k.regs r :=
 by simp [EA.readq, EA.read_reg_64]
 
 theorem EA.write_reg_64 {r k q k'} :
-  (EA.EA_r r).write k wsize.Sz64 q k' ↔ k' = k.set_reg r q :=
+  (EA.r r).write k wsize.Sz64 q k' ↔ k' = k.set_reg r q :=
 by split; [{rintro ⟨⟩, refl}, {rintro rfl, constructor}]
 
 theorem EA.writeq_reg_64 {r k q k'} :
-  (EA.EA_r r).writeq k wsize.Sz64 q k' ↔ k' = k.set_reg r q :=
+  (EA.r r).writeq k wsize.Sz64 q k' ↔ k' = k.set_reg r q :=
 by simp [EA.writeq, EA.write_reg_64]
+
+theorem mem.set.read'_exists {p m q w b v}
+  (h1 : mem.read' p m q v) : ∃ v', mem.read' p (m.set w b) q v' :=
+begin
+  induction h1, {exact ⟨_, mem.read'.nil _ _ _⟩},
+  cases h1_ih with v1 ih,
+  rcases h1_a with ⟨_, rfl, h1⟩,
+  exact ⟨_, mem.read'.cons ⟨_, rfl, h1⟩ ih⟩,
+end
+
+theorem mem.write.read'_exists {p m q a v v2 m'}
+  (h1 : mem.read' p m q v) (h2 : mem.write m a v2 m') :
+  ∃ v', mem.read' p m' q v' :=
+begin
+  induction h2 generalizing v, {exact ⟨_, h1⟩},
+  cases h2_a with h3 h4,
+  cases mem.set.read'_exists h1 with v1 h1,
+  exact h2_ih h1,
+end
+
+theorem EA.read.determ {k ea sz w1 w2}
+  (h1 : EA.read k ea sz w1) (h2 : EA.read k ea sz w2) : w1 = w2 :=
+begin
+  cases ea,
+  { exact h1.trans h2.symm },
+  { cases sz, cases sz, all_goals {exact h1.trans h2.symm} },
+  { rcases h1 with ⟨_, a1, b1⟩,
+    rcases h2 with ⟨_, a2, b2⟩,
+    cases a1.determ_len a2 (b1.1.trans b2.1.symm),
+    exact bits_to_byte.determ_l b1 b2 },
+end
+
+theorem EA.readq.determ {k ea sz q1 q2} :
+  EA.readq k ea sz q1 → EA.readq k ea sz q2 → q1 = q2
+| ⟨a1, b1, e1⟩ ⟨a2, b2, e2⟩ :=
+  by cases b1.determ b2; exact e1.trans e2.symm
+
+theorem hoare_p.bind {P P' : kcfg → Prop}
+  (H : ∀ {{k}}, P k → hoare_p P' k) {k} : hoare_p P k → hoare_p P' k :=
+begin
+  intro h, induction h,
+  exact H h_a,
+  exact hoare_p.step h_a (λ k', h_ih _),
+  by_cases h_ret = 0,
+  { cases H (h_a_1 h),
+    { exact hoare_p.zero a },
+    { cases a with k' h, cases h.no_exit h_a },
+    { exact hoare_p.exit _ _ a a_1 } },
+  { exact hoare_p.exit _ _ h_a h.elim },
+end
+
+theorem hoare_p.mono {P P' : kcfg → Prop}
+  (H : ∀ {{k}}, P k → P' k) {k} : hoare_p P k → hoare_p P' k :=
+hoare_p.bind (λ k h, hoare_p.zero (H h))
 
 end x86
